systems/Log.v
@@ -14,63 +14,127 @@ Section Log.
   Context {l_name_serializer : Serializer name}.
   Context {msg_serializer : Serializer msg}.
   Context {input_serializer : Serializer input}.
+  Context {snapshot_interval : nat}.
 
-  (* entry serializer *)
-  Notation "a +++ b" := (IOStreamWriter.append (fun _ => a) (fun _ => b))
-                      (at level 100, right associativity).
-  Inductive entry : Type :=
-  | LogInput : input -> entry
-  | LogMsg : name * msg -> entry
-  | Reboot : entry.
+  Definition entry : Type := input + (name * msg).
 
-  Definition entry_serialize e :=
-    match e with
-    | LogInput inp => serialize x00 +++ serialize inp
-    | LogMsg nm => serialize x01 +++ serialize nm
-    | Reboot => serialize x02
-    end.
+  Inductive log_files :=
+  | Count
+  | Snapshot
+  | Log.
 
-  Definition entry_deserialize : ByteListReader.t entry :=
-    tag <- deserialize;;
-        match tag with
-        | x00 => LogInput <$> deserialize
-        | x01 => LogMsg <$> deserialize
-        | x02 => ByteListReader.ret Reboot
-        | _ => ByteListReader.error
-        end.
-
-  Lemma entry_serialize_deserialize_id :
-    serialize_deserialize_id_spec entry_serialize entry_deserialize.
+  Lemma log_files_eq_dec : forall x y : log_files, {x = y} + {x <> y}.
   Proof.
-    intros.
-    unfold entry_deserialize, entry_serialize.
-    destruct a;
-      cheerios_crush;
-      simpl;
-      cheerios_crush.
+    decide equality.
   Qed.
 
-  Instance entry_Serializer : Serializer entry.
+  Record log_state := mk_log_state { log_num_entries : nat ;
+                                     log_data : data}.
+
+  Definition log_state_serialize d :=
+    IOStreamWriter.append (fun _ => serialize (log_num_entries d))
+                          (fun _ => serialize (log_data d)).
+
+  Definition log_state_deserialize :=
+    n <- deserialize;;
+      d <- deserialize;;
+      ByteListReader.ret (mk_log_state n d).
+
+  Lemma log_state_serialize_deserialize_id:
+    serialize_deserialize_id_spec log_state_serialize log_state_deserialize.
   Proof.
-    exact {| serialize := entry_serialize;
-             deserialize := entry_deserialize;
-             serialize_deserialize_id := entry_serialize_deserialize_id
+    intros.
+    unfold log_state_serialize, log_state_deserialize.
+    destruct a.
+    cheerios_crush.
+  Qed.
+
+  Instance log_state_Serializer : Serializer log_state.
+  Proof.
+    exact {| serialize := log_state_serialize ;
+             deserialize := log_state_deserialize ;
+             serialize_deserialize_id := log_state_serialize_deserialize_id
           |}.
   Qed.
 
-  Definition log_net_handlers dst src m st : IOStreamWriter.t *
+  Definition log_net_handlers dst src m st : list (disk_op log_files) *
                                              list output *
-                                             data *
+                                             log_state *
                                              list (name * msg)  :=
-    let '(out, data, ps) := net_handlers dst src m st in
-    (serialize (inr (src , m)), out, data, ps).
+    let '(out, data, ps) := net_handlers dst src m (log_data st) in
+    if S (log_num_entries st) =? snapshot_interval
+    then ([Delete Log; Write Snapshot (serialize data)],
+          out,
+          mk_log_state 0 data,
+          ps)
+    else ([Append Log (serialize (inr (src , m)))],
+          out,
+          mk_log_state 0 data,
+          ps).
 
-  Definition log_input_handlers h inp st : IOStreamWriter.t *
+  Definition log_input_handlers h inp st : list (disk_op log_files) *
                                            list output *
-                                           data *
+                                           log_state *
                                            list (name * msg) :=
-    let '(out, data, ps) := input_handlers h inp st in
-    (serialize (inl inp), out, data, ps).
+    let '(out, data, ps) := input_handlers h inp (log_data st) in
+    if S (log_num_entries st) =? snapshot_interval
+    then ([Delete Log; Write Snapshot (serialize data)],
+          out,
+          mk_log_state 0 data,
+          ps)
+    else ([Append Log (serialize (inl inp))],
+          out,
+          mk_log_state 0 data,
+          ps).
+
+  Instance log_base_params : BaseParams :=
+    {
+      data := log_state ;
+      input := input ;
+      output := output
+    }.
+
+  Definition log_init_handlers h :=
+    mk_log_state 0 (init_handlers h).
+
+  Definition init_disk (h : name) : do_disk log_files :=
+    fun file =>
+      match file with
+      | Count => serialize 0
+      | Snapshot => serialize (init_handlers h)
+      | Log => IOStreamWriter.empty
+      end.
+
+  Instance log_multi_params : DiskOpMultiParams log_base_params :=
+    {
+      do_name := name;
+      file_name := log_files;
+      do_name_eq_dec := name_eq_dec;
+      do_msg := msg;
+      do_msg_eq_dec := msg_eq_dec;
+      file_name_eq_dec := log_files_eq_dec;
+      do_nodes := nodes;
+      do_all_names_nodes := all_names_nodes;
+      do_no_dup_nodes := no_dup_nodes;
+      do_init_handlers := log_init_handlers;
+      do_init_disk := init_disk;
+      do_net_handlers := log_net_handlers;
+      do_input_handlers := log_input_handlers
+    }.
+
+  Definition wire_to_log (w : file_name -> IOStreamWriter.wire) : option (nat * @data orig_base_params * list entry) :=
+    match deserialize_top deserialize (w Count) with
+    | Some n =>
+      match deserialize_top deserialize (w Snapshot) with
+      | Some d =>
+        match deserialize_top (list_deserialize_rec _ _ n) (w Log) with
+        | Some es => Some (n, d, es)
+        | None => None
+        end
+      | None => None
+      end
+    | None => None
+    end.
 
   Fixpoint apply_log h (d : data) (entries : list entry) : data :=
     match entries with
@@ -78,72 +142,30 @@ Section Log.
     | e :: entries =>
       apply_log h
                 (match e with
-                 | LogInput inp => match log_input_handlers h inp d with
+                 | inl inp => match log_input_handlers h inp d with
                               | (_, _, d, _) => d
                                    end
-                 | LogMsg (src, m) =>  match log_net_handlers h src m d with
+                 | inr (src, m) =>  match log_net_handlers h src m d with
                                        | (_, _, d, _) => d
-                                       end
-                 | Reboot => reboot d
+                                    end
                  end)
                 entries
     end.
 
-  Instance log_base_params : BaseParams :=
-    {
-      data := data ;
-      input := input ;
-      output := output
-    }.
-
-  Definition init_log h :=
-    (serialize 0, serialize (init_handlers h), list_serialize_rec (input + name * msg) _ []).
-
-  Instance log_multi_params : LogMultiParams log_base_params :=
-    {
-      l_name := name;
-      l_name_eq_dec := name_eq_dec;
-      l_msg := msg;
-      l_msg_eq_dec := msg_eq_dec;
-      l_nodes := nodes;
-      l_all_names_nodes := all_names_nodes;
-      l_no_dup_nodes := no_dup_nodes;
-      l_init_handlers := init_handlers;
-      l_init_log := init_log;
-      l_net_handlers := log_net_handlers;
-      l_input_handlers := log_input_handlers
-    }.
-
-  Definition wire_to_log lw : option (nat * data * list entry) :=
-    match lw with
-    | (nw, dw, ew) =>
-      match deserialize_top deserialize nw with
-      | Some n =>
-        match deserialize_top deserialize dw with
-        | Some d =>
-          match deserialize_top (list_deserialize_rec _ _ n) ew with
-          | Some entries => Some (n, d, entries)
-          | None => None
-          end
-        | None => None
-        end
-      | None => None
-      end
+  Definition do_reboot (h : do_name) (w : log_files -> IOStreamWriter.wire) :
+    (data * do_disk log_files) :=
+    match wire_to_log w with
+    | Some (n, d, es) => (apply_log h (mk_log_state n d) es,
+                          fun file => match file with
+                                      | Count => serialize 0
+                                      | Snapshot => serialize d
+                                      | Log => IOStreamWriter.empty
+                                         end)
+    | None => (mk_log_state 0 (init_handlers h), fun _ => IOStreamWriter.empty)
     end.
 
-  Definition deserialize_apply_log h lw :=
-    match wire_to_log lw with
-    | Some (n, d, entries) => apply_log h d entries
-    | None => l_init_handlers h
-    end.
-
-  Instance log_failure_params : LogFailureParams log_multi_params :=
-    {
-      l_reboot :=
-        fun h lw =>
-          @reboot _ _ orig_failure_params
-                  (deserialize_apply_log h lw)
-    }.
+  Instance log_failure_params : DiskOpFailureParams log_multi_params :=
+    { do_reboot := do_reboot }.
 End Log.
 
 Hint Extern 5 (@BaseParams) => apply log_base_params : typeclass_instances.
