systems/LogCorrect.v
@@ -13,125 +13,65 @@ Section LogCorrect.
   Context {msg_serializer : Serializer msg}.
   Context {input_serializer : Serializer input}.
 
+  Context {snapshot_interval : nat}.
   Hypothesis reboot_idem : forall d, reboot (reboot d) = reboot d.
 
-  Lemma g :
-    @deserialize_top
-            (list entry)
-            (list_deserialize_rec entry entry_Serializer 0)
-            (serialize_top IOStreamWriter.empty) = Some [].
+  Lemma f :
+    deserialize_top
+             (list_deserialize_rec entry
+                (sum_Serializer input (name * msg) input_serializer
+                   (pair_Serializer name msg l_name_serializer msg_serializer)) 0)
+             (serialize_top IOStreamWriter.empty) = Some [].
   Proof.
-    apply serialize_deserialize_top_id' with (bytes := []).
-    unfold list_deserialize_rec.
+    unfold deserialize_top, serialize_top.
+    simpl.
     cheerios_crush.
   Qed.
 
-  Lemma disk_follows_local_state : forall net failed tr h,
-      @step_failure_log_star _ _ log_failure_params step_failure_log_init (failed, net) tr ->
-      (@deserialize_apply_log _
-                              orig_multi_params
-                              _ _ _ _ _
-                              h
-                              (log_to_wire (nwlLog net h))) =
-      (nwlState net h).
+  Lemma disk_follows_local_state : forall net failed tr (h : name) d dsk,
+      @step_failure_log_star _ _
+                             (log_failure_params (snapshot_interval := snapshot_interval)) step_failure_log_init (failed, net) tr ->
+      (do_reboot (snapshot_interval := snapshot_interval))
+        h (disk_to_wire (nwdoDisk net h)) = (d, dsk) ->
+      d = nwdoState net h.
   Proof.
     intros.
     remember step_failure_log_init as x.
+    generalize dependent d. generalize dependent dsk.
     change net with (snd (failed, net)).
     induction H using refl_trans_1n_trace_n1_ind.
     - intros.
-      find_rewrite.
-      simpl.
-      unfold deserialize_apply_log.
-      repeat break_match.
-      + unfold wire_to_log in *.
-        repeat break_match; try congruence.
-        symmetry in Heqo. find_inversion.
-        rewrite serialize_deserialize_top_id in Heqo0.
-        rewrite serialize_deserialize_top_id in Heqo1.
-        repeat find_inversion.
-        rewrite g in *.
+      rewrite Heqx in *.
+      simpl in *.
+      unfold disk_to_wire, init_disk, do_reboot in *.
+      break_match;
+        unfold wire_to_log in *;
+        repeat rewrite serialize_deserialize_top_id in Heqo;
+        rewrite f in *.
+      + break_let.
+        break_let.
+        find_inversion.
         find_inversion.
         reflexivity.
-      + reflexivity.
+      + congruence.
     - concludes.
-      destruct H0.
-      + destruct net'.
-        simpl in *.
-        inversion H5.
-        break_if.
-        * unfold update_log in *.
-          unfold log_net_handlers in *.
-          repeat break_match.
-          -- repeat tuple_inversion.
-             match goal with
-             | H : _ = Some log |- _ => inversion H
-             end.
-             unfold deserialize_apply_log.
-             repeat break_match.
-             ++ admit.
-             ++ unfold log_to_wire, wire_to_log in *.
-                repeat break_match; try congruence; admit.
-          -- inversion H4.
-             unfold deserialize_apply_log.
-             repeat break_match;
-               admit.
-          -- inversion H4.
-        * assumption.
-      + destruct net'.
-        simpl in *.
-        inversion H5.
-        break_if.
-        * unfold deserialize_apply_log.
-          repeat break_match.
-          --
-             admit.
-          -- admit.
-        * assumption.
-      + destruct net0 eqn:Hnet0.
-        simpl in *.
-        assert (Net.nwlLog net' = nwlLog). match goal with
-                                           | H : net' = _ |- _ => now rewrite H
-                                           end.
-        assert (Net.nwlState net' = nwlState). match goal with
-                                               | H : net' = _ |- _ => now rewrite H
-                                               end.
-        * now repeat find_rewrite.
-      + destruct net0 eqn:Hnet0.
-        simpl in *.
-        assert (Net.nwlLog net' = nwlLog). match goal with
-                                           | H : net' = _ |- _ => now rewrite H
-                                           end.
-        assert (Net.nwlState net' = nwlState). match goal with
-                                               | H : net' = _ |- _ => now rewrite H
-                                               end.
-        * now repeat find_rewrite.
-      + assumption.
-      + simpl in H3. simpl.
-        destruct net'.
-        inversion H4.
-        simpl in *.
-         break_if.
-        * rewrite <- H3.
-          rewrite e in *.
-          rewrite IHrefl_trans_1n_trace1.
-          symmetry.
-          apply reboot_idem.
-         * assumption.
+      rewrite Heqx in *.
+      admit.
   Admitted.
 
   Definition orig_packet := @packet _ orig_multi_params.
   Definition orig_network := @network _ orig_multi_params.
 
-  Definition log_packet := @l_packet _ log_multi_params.
-  Definition log_network := @l_network _ log_multi_params.
+  Definition log_packet := @do_packet _ (log_multi_params (snapshot_interval := snapshot_interval)).
+  Definition log_network := @do_network _ (log_multi_params (snapshot_interval := snapshot_interval)).
 
 
   Definition revertPacket (p : log_packet) : orig_packet :=
-    @mkPacket _ orig_multi_params (l_pSrc p) (l_pDst p) (l_pBody p).
+    @mkPacket _ orig_multi_params (do_pSrc p) (do_pDst p) (do_pBody p).
 
   Definition revertLogNetwork (net: log_network) : orig_network :=
-    mkNetwork (map revertPacket (nwlPackets net)) (nwlState net).
+    mkNetwork (map revertPacket (nwdoPackets net))
+              (fun h => (log_data (nwdoState net h))).
 
   Theorem disk_step_failure_step :
     forall net net' failed failed' tr tr',
@@ -143,75 +83,15 @@ Section LogCorrect.
   Proof.
     intros.
     assert (revert_packets : forall net, nwPackets (revertLogNetwork net) =
-                        map revertPacket (nwlPackets net)) by reflexivity.
+                        map revertPacket (nwdoPackets net)) by reflexivity.
     assert (revert_send : forall l h,
-               map revertPacket (l_send_packets h l) = send_packets h l).
+               map revertPacket (do_send_packets h l) = send_packets h l).
       { induction l.
         * reflexivity.
         * intros.
           simpl.
           now rewrite IHl.
       }
-    invcs H0.
-    - unfold revertLogNetwork in *.
-      simpl.
-      repeat find_rewrite.
-      rewrite map_app.
-      simpl in *. unfold log_net_handlers in *.
-      repeat break_let. simpl.
-      assert (l_pDst p = pDst (revertPacket p)) by reflexivity.
-      repeat find_rewrite.
-      find_inversion.
-      repeat rewrite map_app.
-
-      apply StepFailure_deliver with (xs0 := map revertPacket xs)
-                                     (ys0 := map revertPacket ys)
-                                     (d0 := d)
-                                     (l0 := l).
-      + reflexivity.
-      + assumption.
-      + assumption.
-      + simpl.
-        now rewrite revert_send.
-    - unfold revertLogNetwork in *. simpl. repeat find_rewrite.
-      simpl in *. unfold log_input_handlers in *.
-      repeat break_let. find_inversion.
-      rewrite map_app.
-      rewrite revert_send.
-      match goal with
-      | H : input_handlers _ _ _ = (_, ?d, ?l) |- _ =>
-        apply StepFailure_input with (d0 := d) (l0 := l); auto
-      end.
-    - unfold revertLogNetwork.
-      simpl.
-      find_rewrite.
-      repeat rewrite map_app.
-      simpl.
-      match goal with
-      | H : _ = ?xs ++ ?p :: ?ys |- _ =>
-        apply StepFailure_drop with (p0 := revertPacket p)
-                                    (xs0 :=  map revertPacket xs)
-                                    (ys0 := map revertPacket ys)
-      end; reflexivity.
-    - unfold revertLogNetwork.
-      match goal with H : nwlPackets net = _ |- _ => rewrite H end.
-      rewrite map_app. simpl.
-      match goal with
-      | H : _ = ?xs ++ ?p :: ?ys |- _ =>
-        apply StepFailure_dup with (p0 := revertPacket p)
-                                   (xs0 :=  map revertPacket xs)
-                                   (ys0 := map revertPacket ys)
-      end.
-      + reflexivity.
-      + now rewrite map_app.
-    - apply (@StepFailure_fail _ _ orig_failure_params).
-    - match goal with
-        H : In ?h _ |- _ => apply StepFailure_reboot with (h0 := h)
-      end.
-      + assumption.
-      + reflexivity.
-      + unfold revertLogNetwork. simpl.
-        rewrite (disk_follows_local_state _ failed tr);
-          auto.
-  Qed.
+      invcs H0.
+      Admitted.
 End LogCorrect.
